ott/coq/Context.v
@@ -1,351 +1,59 @@
-Require Import Bool List.
-
 Require Import Common.
 
-Definition add {A B} (E : list (A * B)) a b :=
-  (a, b) :: E.
+Definition context (A B : Set) := list (A * B).
+Arguments context : default implicits.
 
-Inductive Lookup {A B : Type} : list (A * B) -> A -> B -> Type :=
-  | Lookup_hd     a b E :                           Lookup (cons (a,b) E) a b
-  | Lookup_tl x y a b E : x <> a -> Lookup E a b -> Lookup (cons (x,y) E) a b.
+Definition eq_context {A B} eq_A eq_B : context A B -> context A B -> bool :=
+  eq_list (eq_pair eq_A eq_B).
 
-Fixpoint Lookup_unique {A B : Type} E (a : A) (b1 b2 : B) (L1 : Lookup E a b1) (L2 : Lookup E a b2) {struct E} : b1 = b2.
-Proof.
-  destruct E; simple inversion L1; simple inversion L2; try congruence; intros.
-  + match goal with
-    | [L1 : Lookup ?E1 _ _, L2 : Lookup ?E2 _ _ |- _] =>
-        is_var E1; is_var E2;
-        assert (E1 = E) by congruence;
-        assert (E2 = E) by congruence
+Definition add {A B} (C : context A B) a b :=
+  (a, b) :: C.
+
+Definition lookup {A B : Set} (eq_A : A -> A -> bool) :=
+  fix lookup (E : context A B) (a : A) : option B :=
+    match E with
+      | nil          => None
+      | cons (x,b) E => if eq_A x a then Some b
+                                    else lookup E a
     end.
-    eapply (Lookup_unique A B E a b1 b2); subst; eassumption.
-Qed.
 
-Fixpoint lookup_find {A B} (eq : A -> A -> bool) (E : list (A * B)) (a : A) : option B :=
-  match E with
-  | nil          => None
-  | cons (x,b) E => if eq x a then Some b
-                              else lookup_find eq E a
-  end.
-
-Fixpoint lookup_find_correct {A B} {eq : A -> A -> bool} (E : list (A * B)) (a : A) {struct E} :
-  (forall x y, boolSpec (eq x y) (x = y)) ->
-  match lookup_find eq E a with
-  | Some b => Lookup E a b
-  | None   => forall b, neg (Lookup E a b)
-  end.
-Proof.
-  intros eq_correct.
-  unfold_goal.
-  destruct E; simpl.
-  + intros ?; inversion 1.
-  + destruct p as [x b]; simpl.
-    set (eq_correct x a).
-    case_eq (eq x a); boolSpec_simpl; simpl.
-    - my_auto.
-    - fold (lookup_find eq E a).
-      set (lookup_find_correct A B eq E a eq_correct).
-      case_eq (lookup_find eq E a).
-      * intros ? Heq.
-        rewrite Heq in *; my_auto.
-      * intros Heq.
-        rewrite Heq in *.
-        intros ?; inversion 1; firstorder.
-Defined.
-
-Fixpoint lookup_find_unique {A B} {eq : A -> A -> bool} (E : list (A * B)) (a : A) (b : B) {struct E} :
-  (forall x y, boolSpec (eq x y) (x = y)) ->
-  Lookup E a b ->
-  lookup_find eq E a = Some b.
-Proof.
-  intros eq_correct.
-  destruct E.
-  + my_auto.
-  + inversion 1; simpl; set (eq_correct a a); boolSpec_destruct; my_auto.
-    set (eq_correct x a); boolSpec_simpl; my_auto.
-Defined.
-
-Definition Disjoint {A B1 B2} E1 E2 : Type :=
-  forall (a : A) (b1 : B1) (b2 : B2), Lookup E1 a b1 -> Lookup E2 a b2 -> False.
-
-Definition env_sub {A B} (P : A -> Type) (E1 E2 : list (A * B)) :=
-  forall id, P id -> forall b, Lookup E1 id b -> Lookup E2 id b.
-
-Definition env_equiv {A B} (P : A -> Type) (E1 E2 : list (A * B)) :=
-  env_sub P E1 E2 * env_sub P E2 E1.
-
-Lemma Disjoint_cons_left_Lookup {A B C} {a} {b} {E1 : list (A * B)} {E : list (A * C)} :
-  Disjoint ((a,b) :: E1) E -> forall c, neg (Lookup E a c).
-Proof.
-  intros Hdisjoint.
-  assert (Lookup ((a,b) :: E1) a b) as Hlookup by constructor.
-  exact (fun c => Hdisjoint a b c Hlookup).
-Qed.
-
-Lemma Disjoint_cons_left_Lookup_inv {A B C} {a} {b} {E1 : list (A * B)} {E : list (A * C)} :
-  Disjoint E1 E -> (forall c, neg (Lookup E a c)) -> Disjoint ((a,b) :: E1) E.
-Proof.
-  intros Hdisjoint Hnlookup.
-  intros a' b' c'.
-  inversion 1; subst.
-  - apply Hnlookup.
-  - eapply Hdisjoint.
-    eassumption.
-Qed.
-
-Lemma Disjoint_cons_left {A B C} p {E1 E2 : list (A * B)} {E : list (A * C)} :
-  Disjoint (p :: E1) E -> Disjoint E2 E -> Disjoint (p :: E2) E.
-Proof.
-  intros; destruct p.
-  eapply Disjoint_cons_left_Lookup_inv.
-  - assumption.
-  - eapply Disjoint_cons_left_Lookup; eassumption.
-Qed.
-
-Lemma Disjoint_weaken {A B C} {eq_dec : DecidableEq A} {p} {E1 : list (A * B)} {E : list (A * C)}:
-  Disjoint (p :: E1) E ->
-  Disjoint E1 E.
-Proof.
-  destruct p.
-  intros Hdisjoint a' b' c' Hlookup.
-  destruct (decide a a' : Decision (a = a')).
-  + subst.
-    eapply (Hdisjoint a').
-    constructor 1.
-  + eapply (Hdisjoint a').
-    constructor 2; eassumption.
-Qed.  
-
-Lemma Disjoint_app {A B C} {eq_dec : DecidableEq A} {E1 E2 : list (A * B)} {E : list (A * C)}:
-  Disjoint E1 E ->
-  Disjoint E2 E ->
-  Disjoint (E1++E2) E.
-Proof.
-  induction E1.
-  - intros; assumption.
-  - intros H1 H2.
-    assert (Disjoint E1 E) as H
-      by (eapply Disjoint_weaken; eassumption).
-    eapply Disjoint_cons_left.
-    + eassumption.
-    + exact (IHE1 H H2).
-Qed.
-
-Definition context_ind {A B} (P : list (A * B) -> Type) :
-  (P nil) ->
-  (forall a b E, P E -> P (add E a b)) ->
-  (forall E, P E).
-Proof.
-  intros Hnil Hcons.
-  induction E as [|[? ?]].
-  + exact Hnil.
-  + eapply Hcons; assumption.
-Qed.
-
-Inductive linear {A B} : list (A * B) -> Type :=
-  | LinearNil        : linear nil
-  | LinearCons a b E : (forall b, neg (Lookup E a b)) -> linear E -> linear ((a, b) :: E).
-
-Fixpoint remove_var_fun {A B} (eq_fun : A -> A -> bool) a E : list (A * B) :=
-  match E with
+Fixpoint remove_var {A B: Set} (eq_A : A -> A -> bool) a C : context A B :=
+  match C with
   | nil             => nil
-  | cons (a', b') E => if eq_fun a a' 
-                         then remove_var_fun eq_fun a E
-                         else (a', b') :: remove_var_fun eq_fun a E
+  | cons (a', b') C => if eq_A a a' 
+                         then remove_var eq_A a C
+                         else (a', b') :: remove_var eq_A a C
   end.
 
-Lemma remove_var_fun_complete {A B} (eq_fun : A -> A -> bool) a (E : list (A * B)) :
-  (forall x y, boolSpec (eq_fun x y) (x = y)) ->
-  forall a' b', 
-    neg (a = a') ->
-    Lookup E a' b' ->
-    Lookup (remove_var_fun eq_fun a E) a' b'.
-Proof.
-  intros eq_fun_correct.
-  induction E as [|[? ?] E IH]; simpl.
-  - inversion 2.
-  - inversion 2;
-    match goal with
-    | [|- context[eq_fun ?a1 ?a2]] =>
-        generalize (eq_fun_correct a1 a2);
-        destruct (eq_fun a1 a2)
-    end; my_auto.
-Qed.
-
-Lemma remove_var_fun_sound {A B} (eq_fun : A -> A -> bool) a (E : list (A * B)) :
-  (forall x y, boolSpec (eq_fun x y) (x = y)) ->
-  forall a' b', 
-    neg (a = a') ->
-    Lookup (remove_var_fun eq_fun a E) a' b' ->
-    Lookup E a' b'.
-Proof.
-  intros eq_fun_correct ? ? ?.
-  induction E as [|[? ?] E IH]; simpl.
-  - inversion 1.
-  - match goal with
-    | [|- context[eq_fun ?a1 ?a2]] =>
-        generalize (eq_fun_correct a1 a2);
-        destruct (eq_fun a1 a2);
-        simpl
-    end.
-    + intros;      my_auto.
-    + inversion 2; my_auto.
-Qed.
-
-Lemma remove_var_fun_Lookup {A B} (eq_fun : A -> A -> bool) a (E : list (A * B)) :
-  (forall x y, boolSpec (eq_fun x y) (x = y)) ->
-  forall b, neg (Lookup (remove_var_fun eq_fun a E) a b).
-Proof.
-  intros eq_fun_correct.
-  induction E as [|[? ?] E IH]; simpl.
-  - inversion 1.
-  - match goal with
-    | [|- context[eq_fun ?a1 ?a2]] =>
-        generalize (eq_fun_correct a1 a2);
-        destruct (eq_fun a1 a2);
-        simpl
-    end.
-    + my_auto.
-    + inversion 2.
-      * my_auto.
-      * firstorder.
-Qed.
-
-Fixpoint linearize_fun {A B} (eq_fun : A -> A -> bool) E : list (A * B) :=
-  match E with
-  | nil           => nil
-  | cons (a, b) E => cons (a, b) (remove_var_fun eq_fun a (linearize_fun eq_fun E))
+Fixpoint linearize {A B: Set} (eq_A : A -> A -> bool) C : context A B :=
+  match C with
+  | nil         => nil
+  | (a, b) :: C => (a, b) :: remove_var eq_A a (linearize eq_A C)
   end.
 
-Lemma linearize_fun_sound {A B} {eq_fun : A -> A -> bool} (E : list (A * B)) :
-  (forall x y, boolSpec (eq_fun x y) (x = y)) ->
-  forall a' b',
-    Lookup (linearize_fun eq_fun E) a' b' ->
-    Lookup E a' b'.
-Proof.
-  intros eq_fun_correct.
-  induction E as [|[? ?]]; simpl.
-  - inversion 1.
-  - inversion 1; subst.
-    + constructor.
-    + constructor 2.
-      * assumption.
-      * apply IHE.
-        eapply remove_var_fun_sound; eassumption.
-Qed.
-
-Lemma linearize_fun_complete {A B} {eq_fun : A -> A -> bool} (E : list (A * B)) :
-  (forall x y, boolSpec (eq_fun x y) (x = y)) ->
-  forall a' b',
-    Lookup E a' b' ->
-    Lookup (linearize_fun eq_fun E) a' b'.
-Proof.
-  intros eq_fun_correct.
-  induction E as [|[? ?]]; simpl.
-  - inversion 1.
-  - inversion 1; subst.
-    + constructor.
-    + constructor 2.
-      * assumption.
-      * eapply remove_var_fun_complete; my_auto.
-Qed.  
-
-Lemma linear_remove_var_fun {A B} {eq_fun : A -> A -> bool} a (E : list (A * B)) :
-  (forall x y, boolSpec (eq_fun x y) (x = y)) ->
-  linear E -> linear (remove_var_fun eq_fun a E).
-Proof.
-  intros eq_fun_correct.
-  induction E as [|[? ?]]; simpl.
-  - my_auto.
-  - match goal with
-    | [|- context[eq_fun ?a1 ?a2] ] =>
-        generalize (eq_fun_correct a1 a2);
-        destruct (eq_fun a1 a2);
-        simpl; intros ?
-    end.
-    + inversion 1; my_auto.
-    + inversion 1; subst.
-      constructor.
-      * intros ? ?.
-        match goal with
-        | [H : forall _, neg (Lookup E _ _) |- _] =>
-            eapply H;
-            eapply remove_var_fun_sound;
-            eassumption
-        end.
-      * my_auto.
-Qed.
-
-Lemma linearize_fun_linear {A B} {eq_fun : A -> A -> bool} (E : list (A * B)) :
-  (forall x y, boolSpec (eq_fun x y) (x = y)) ->  
-  linear (linearize_fun eq_fun E).
-Proof.
-  intros eq_fun_correct.
-  induction E as [|[? ?]]; simpl.
-  - constructor.
-  - econstructor.
-    + apply remove_var_fun_Lookup; assumption.
-    + apply linear_remove_var_fun; assumption.
-Qed.
-
-Fixpoint context_linear_all_fun {A B} (eq_fun : A -> A -> bool) (P_fun : A -> B -> bool) E : bool :=
-  match E with
-  | nil           => true
-  | cons (a, b) E => andb (P_fun a b) (context_linear_all_fun eq_fun P_fun E)
+Fixpoint all_linear {A B: Set} (eq_A : A -> A -> bool) (p : A -> B -> bool) C : bool :=
+  match C with
+  | nil         => true
+  | (a, b) :: C => p a b && all_linear eq_A p C
   end.
 
-Fixpoint context_linear_all_fun_correct {A B} {eq_fun : A -> A -> bool} {P_fun : A -> B -> bool} {P : A -> B -> Type} {E} :
-  (forall x y, boolSpec (eq_fun x y) (x = y)) ->
-  (forall x y, boolSpec (P_fun  x y) (P x y)) ->
-  linear E ->
-  boolSpec (context_linear_all_fun eq_fun P_fun E) (forall a b, Lookup E a b -> P a b).
-Proof.
-  intros eq_fun_correct P_fun_correct.
-  induction E as [| [a b] E IH]; simpl.
-  - my_auto.
-  - match goal with
-    | [|- context[P_fun ?a1 ?a2] ] =>
-        generalize (P_fun_correct a1 a2);
-        destruct (P_fun a1 a2);
-        simpl; [intros ?| intros P_neg]
-    end.
-    + inversion 1 as [| ? ? ? Hfalse Hlinear]; subst.
-      match goal with
-      | [|- context[context_linear_all_fun eq_fun P_fun ?E] ] =>
-          generalize (context_linear_all_fun_correct _ _ _ _ _ E eq_fun_correct P_fun_correct Hlinear);
-          destruct (context_linear_all_fun eq_fun P_fun E);
-          simpl; intros ?
-      end.
-      inversion 1; my_auto.
-      intros Hlookup.
-      apply (IH Hlinear); intros.
-      apply Hlookup.
-      constructor 2.
-      * intros ?; subst; firstorder.
-      * assumption.
-    + intros Hlinear Hfalse.
-      apply P_neg.
-      apply Hfalse.
-      constructor.
-Qed.
+Definition all {A B: Set} (eq_A : A -> A -> bool) (p : A -> B -> bool) C : bool :=
+  all_linear eq_A p (linearize eq_A C).
 
-Definition context_all_fun {A B} (eq_fun : A -> A -> bool) (P_fun : A -> B -> bool) E : bool :=
-  context_linear_all_fun eq_fun P_fun (linearize_fun eq_fun E).
+Definition sub_p {A B: Set} (eq_A : A -> A -> bool) (p : A -> bool) (equiv_B : B -> B -> bool) (C1 C2 : context A B) :=
+  all eq_A (fun a b =>
+              if p a
+                then match lookup eq_A C2 a with
+                     | Some b' => equiv_B b b'
+                     | None    => false
+                     end
+                else true) C1.
 
-Lemma context_all_fun_correct {A B} {eq_fun : A -> A -> bool} {P_fun : A -> B -> bool} {P : A -> B -> Type} E :
-  (forall x y, boolSpec (eq_fun x y) (x = y)) ->
-  (forall x y, boolSpec (P_fun  x y) (P x y)) ->
-  boolSpec (context_all_fun eq_fun P_fun E) (forall a b, Lookup E a b -> P a b).
-Proof.
-  intros eq_fun_correct P_fun_correct.
-  do 2 unfold_goal.
-  generalize (context_linear_all_fun_correct eq_fun_correct P_fun_correct (linearize_fun_linear E eq_fun_correct)).
-  destruct (context_linear_all_fun eq_fun P_fun (linearize_fun eq_fun E)); simpl; intros H.
-  - intros.
-    apply H.
-    apply linearize_fun_complete; assumption.
-  - intros Hlookup.
-    apply H; intros.
-    apply Hlookup.
-    eapply linearize_fun_sound; eassumption.
-Qed.
+Definition sub {A B: Set} (eq_A : A -> A -> bool) (equiv_B : B -> B -> bool) :=
+  sub_p eq_A (fun _ => true) equiv_B.
+
+Definition equiv_p {A B: Set} (eq_A : A -> A -> bool) (p : A -> bool) (equiv_B : B -> B -> bool) (C1 C2 : context A B) :=
+  sub_p eq_A p equiv_B C1 C2 && sub_p eq_A p equiv_B C2 C1.
+
+Definition equiv {A B: Set} (eq_A : A -> A -> bool) (equiv_B : B -> B -> bool)  (C1 C2 : context A B) :=
+  sub eq_A equiv_B C1 C2 && sub eq_A equiv_B C2 C1.
